eve/Src/examples/proofs/presentation/command/command_test.e
@@ -11,10 +11,13 @@ feature
 
 	make
 		local
-			c1, c2: COMMAND
+			c1: COMMAND
+			ac: ACCOUNT_COMMAND
 			u1: UNDO_COMMAND
 			b: ACCOUNT
 			ca: CREDIT_ACCOUNT
+
+
 		do
 			create b.make
 			create ca.make (200)
@@ -22,22 +25,29 @@ feature
 			create u1.make_undo (agent ca.deposit, agent ca.withdraw, 50)
 			create c1.make (agent b.withdraw, 10)
 
-			check
-				ca.balance = 0
-			end
+			create ac.make (agent {ACCOUNT}.withdraw)
 
-			u1.execute_undo (50)
+			b.deposit (100)
 
-			check
-				ca.balance = -50
-				ca.credit_limit = 200
-			end
+			ac.execute (b, 10)
 
-			u1.execute_undo (50)
 
-			check
-				ca.balance = -100
-			end
+--			check
+--				ca.balance = 0
+--			end
+
+--			u1.execute_undo (50)
+
+--			check
+--				ca.balance = -50
+--				ca.credit_limit = 200
+--			end
+
+--			u1.execute_undo (50)
+
+--			check
+--				ca.balance = -100
+--			end
 
 
 		end
