eve/Src/examples/proofs/presentation/strategy/strategy_test.e
@@ -1,0 +1,36 @@
+indexing
+	description: "Summary description for {STRATEGY_TEST}."
+	author: ""
+	date: "$Date$"
+	revision: "$Revision$"
+
+class
+	STRATEGY_TEST
+
+feature
+
+	test
+		local
+			c: CONTEXT
+			t: INTEGER
+		do
+
+			create c.set_strategy (create {ADDITION_STRATEGY})
+
+			c.execute (1, 2)
+
+			check
+				c.last_result = 3
+			end
+
+			c.set_strategy (create {SUBTRACTION_STRATEGY})
+
+			c.execute (1, 2)
+
+			check
+				c.last_result = -1
+			end
+
+		end
+
+end
